src/Narcissus/BinLib/AlignedSumType.v
@@ -7,6 +7,7 @@ Require Import
         Fiat.Common.SumType
         Fiat.Common.BoundedLookup
         Fiat.Common.ilist
+        Fiat.Common.i2list
         Fiat.Common.DecideableEnsembles
         Fiat.Common.IterateBoundedIndex
         Fiat.Computation
@@ -24,25 +25,111 @@ Section AlignedSumType.
   Context {cache : Cache}.
   Context {cacheAddNat : CacheAdd cache nat}.
 
+  Definition align_format_sumtype
+             {m : nat}
+             {types : t Type m}
+             (align_encoders_n :
+                ilist2.ilist2 (B := fun T : Type => T -> CacheFormat -> nat) types)
+             (align_encoders_v :
+                i2list (B := fun T : Type => T -> CacheFormat -> nat)
+                       (fun (T : Type) (n : _) => forall t ce, Vector.t (word 8) (n t ce)) align_encoders_n)
+             (align_encoders_ce :
+                ilist (B := (fun T : Type => T -> CacheFormat -> CacheFormat)) types)
+             (st : SumType types)
+             (ce : CacheFormat)
+    := (existT _ _ (i2th align_encoders_v (SumType_index types st) (SumType_proj types st) ce),
+        ith align_encoders_ce (SumType_index types st) (SumType_proj types st) ce).
+
+  Lemma align_format_sumtype_OK'
+        {m : nat}
+        {types : t Type m}
+        (align_encoders_n :
+           ilist2.ilist2 (B := fun T : Type => T -> CacheFormat -> nat) types)
+        (align_encoders_v :
+           i2list (B := fun T : Type => T -> CacheFormat -> nat)
+                  (fun (T : Type) (n : _) => forall t ce, Vector.t (word 8) (n t ce)) align_encoders_n)
+        (align_encoders_ce :
+           ilist (B := (fun T : Type => T -> CacheFormat -> CacheFormat)) types)
+        (formatrs :
+           ilist (B := (fun T : Type => T -> @CacheFormat cache -> Comp (ByteString * (CacheFormat)))) types)
+        (formatrs_OK : forall idx t (ce : CacheFormat),
+            refine (ith formatrs idx t ce)
+                   (ret (build_aligned_ByteString (i2th align_encoders_v idx t ce),
+                         ith align_encoders_ce idx t ce)))
+    : forall (st : SumType types)
+             (ce : CacheFormat),
+      refine (format_SumType types formatrs st ce)
+             (ret (build_aligned_ByteString (projT2 (fst (align_format_sumtype
+                                                            align_encoders_n
+                                                            align_encoders_v
+                                                            align_encoders_ce st ce))),
+                   (snd (align_format_sumtype align_encoders_n
+                                                            align_encoders_v
+                                                            align_encoders_ce st ce)))).
+  Proof.
+    intros; unfold format_SumType, align_format_sumtype.
+    rewrite formatrs_OK; reflexivity.
+  Qed.
+
+  Corollary align_format_sumtype_OK
+            {m : nat}
+            {types : t Type m}
+            (align_encoders_n :
+               ilist2.ilist2 (B := fun T : Type => T -> CacheFormat -> nat) types)
+            (align_encoders_v :
+               i2list (B := fun T : Type => T -> CacheFormat -> nat)
+                      (fun (T : Type) (n : _) => forall t ce, Vector.t (word 8) (n t ce)) align_encoders_n)
+            (align_encoders_ce :
+               ilist (B := (fun T : Type => T -> CacheFormat -> CacheFormat)) types)
+            (formatrs :
+               ilist (B := (fun T : Type => T -> @CacheFormat cache -> Comp (ByteString * (CacheFormat)))) types)
+            (formatrs_OK : Iterate_Ensemble_BoundedIndex (fun idx => forall t (ce : CacheFormat),
+                                                              refine (ith formatrs idx t ce)
+                                                                         (ret (build_aligned_ByteString (i2th align_encoders_v idx t ce),
+                                                                               ith align_encoders_ce idx t ce))))
+    : forall (st : SumType types)
+             (ce : CacheFormat),
+      refine (format_SumType types formatrs st ce)
+             (ret (build_aligned_ByteString (projT2 (fst (align_format_sumtype align_encoders_n
+                                                                               align_encoders_v
+                                                                               align_encoders_ce st ce))),
+                   (snd (align_format_sumtype align_encoders_n
+                                              align_encoders_v
+                                              align_encoders_ce st ce)))).
+  Proof.
+    intros; eapply align_format_sumtype_OK'; intros.
+    eapply Iterate_Ensemble_BoundedIndex_equiv in formatrs_OK.
+    apply formatrs_OK.
+  Qed.
+
   Lemma align_format_sumtype_OK_inv'
         {m : nat}
         {types : t Type m}
         (A_OKs : SumType types -> Prop)
-        (align_encoders :
-           ilist (B := (fun T : Type => T -> CacheFormat -> ({n : _ & Vector.t (word 8) n} * (CacheFormat)))) types)
+        (align_encoders_n :
+               ilist2.ilist2 (B := fun T : Type => T -> CacheFormat -> nat) types)
+            (align_encoders_v :
+               i2list (B := fun T : Type => T -> CacheFormat -> nat)
+                      (fun (T : Type) (n : _) => forall t ce, Vector.t (word 8) (n t ce)) align_encoders_n)
+            (align_encoders_ce :
+               ilist (B := (fun T : Type => T -> CacheFormat -> CacheFormat)) types)
         (encoders :
            ilist (B := (fun T : Type => T -> CacheFormat -> Comp (ByteString * (CacheFormat)))) types)
         (encoders_OK : forall idx t (ce : CacheFormat),
             A_OKs (inj_SumType _ idx t)
             -> refine (ith encoders idx t ce)
-                      (ret (build_aligned_ByteString (projT2 (fst (ith align_encoders idx t ce))),
-                            snd (ith align_encoders idx t ce))))
+                      (ret (build_aligned_ByteString (i2th align_encoders_v idx t ce),
+                            ith align_encoders_ce idx t ce)))
     : forall (st : SumType types)
              (ce : CacheFormat),
       A_OKs st
       -> refine (format_SumType types encoders st ce)
-                (ret (build_aligned_ByteString (projT2 (fst (align_format_sumtype align_encoders st ce))),
-                      (snd (align_format_sumtype align_encoders st ce)))).
+                (ret (build_aligned_ByteString (projT2 (fst (align_format_sumtype align_encoders_n
+                                                                               align_encoders_v
+                                                                               align_encoders_ce st ce))),
+                      (snd (align_format_sumtype align_encoders_n
+                                                 align_encoders_v
+                                                 align_encoders_ce st ce)))).
   Proof.
     intros; unfold format_SumType, align_format_sumtype.
     rewrite encoders_OK; eauto.
@@ -50,26 +137,35 @@ Section AlignedSumType.
     rewrite inj_SumType_proj_inverse; eauto.
   Qed.
 
-  Corollary align_format_sumtype_OK
+  Corollary align_format_sumtype_OK_inv
             {m : nat}
             {types : t Type m}
             (A_OKs : SumType types -> Prop)
-            (align_encoders :
-               ilist (B := (fun T : Type => T -> CacheFormat -> ({n : _ & Vector.t (word 8) n} * (CacheFormat)))) types)
+            (align_encoders_n :
+               ilist2.ilist2 (B := fun T : Type => T -> CacheFormat -> nat) types)
+            (align_encoders_v :
+               i2list (B := fun T : Type => T -> CacheFormat -> nat)
+                      (fun (T : Type) (n : _) => forall t ce, Vector.t (word 8) (n t ce)) align_encoders_n)
+            (align_encoders_ce :
+               ilist (B := (fun T : Type => T -> CacheFormat -> CacheFormat)) types)
             (encoders :
                ilist (B := (fun T : Type => T -> CacheFormat -> Comp (ByteString * (CacheFormat)))) types)
             (encoders_OK : Iterate_Ensemble_BoundedIndex
                              (fun idx => forall t (ce : CacheFormat),
                                   A_OKs (inj_SumType _ idx t)
                                   -> refine (ith encoders idx t ce)
-                                            (ret (build_aligned_ByteString (projT2 (fst (ith align_encoders idx t ce))),
-                                                  snd (ith align_encoders idx t ce)))))
+                                            (ret (build_aligned_ByteString (i2th align_encoders_v idx t ce),
+                                                  ith align_encoders_ce idx t ce))))
     : forall (st : SumType types)
              (ce : CacheFormat),
       A_OKs st
       -> refine (format_SumType types encoders st ce)
-                (ret (build_aligned_ByteString (projT2 (fst (align_format_sumtype align_encoders st ce))),
-                      (snd (align_format_sumtype align_encoders st ce)))).
+                (ret (build_aligned_ByteString (projT2 (fst (align_format_sumtype align_encoders_n
+                                                                               align_encoders_v
+                                                                               align_encoders_ce st ce))),
+                      (snd (align_format_sumtype align_encoders_n
+                                                 align_encoders_v
+                                                 align_encoders_ce st ce)))).
   Proof.
     intros; eapply align_format_sumtype_OK_inv'; intros.
     eapply Iterate_Ensemble_BoundedIndex_equiv in encoders_OK.
@@ -80,32 +176,46 @@ Section AlignedSumType.
   Lemma AlignedFormatSumTypeDoneC
             {m : nat}
             {types : t Type m}
-            (A_OKs : SumType types -> Prop)
-            (align_encoders :
-               ilist (B := (fun T : Type => T -> CacheFormat -> ({n : _ & Vector.t (word 8) n} * (CacheFormat)))) types)
+            (A_OKs_l : ilist (B := fun T : Type => T -> Prop) types)
+            (A_OKs : SumType types -> Prop := fun st => ith A_OKs_l (SumType_index _ st) (SumType_proj _ st))
+            (align_encoders_n :
+               ilist2.ilist2 (B := fun T : Type => T -> CacheFormat -> nat) types)
+            (align_encoders_v :
+               i2list (B := fun T : Type => T -> CacheFormat -> nat)
+                      (fun (T : Type) (n : _) => forall t ce, Vector.t (word 8) (n t ce)) align_encoders_n)
+            (align_encoders_ce :
+               ilist (B := (fun T : Type => T -> CacheFormat -> CacheFormat)) types)
             (encoders :
                ilist (B := (fun T : Type => T -> CacheFormat -> Comp (ByteString * (CacheFormat)))) types)
             (encoders_OK : Iterate_Ensemble_BoundedIndex
                              (fun idx => forall t (ce : CacheFormat),
                                   A_OKs (inj_SumType _ idx t)
                                   -> refine (ith encoders idx t ce)
-                                            (ret (build_aligned_ByteString (projT2 (fst (ith align_encoders idx t ce))),
-                                                  snd (ith align_encoders idx t ce)))))
+                                            (ret (build_aligned_ByteString (i2th align_encoders_v idx t ce),
+                                                  ith align_encoders_ce idx t ce))))
     : forall (st : SumType types)
              (ce : CacheFormat),
       A_OKs st
       -> refine (((format_SumType types encoders st) DoneC) ce)
-                (ret (build_aligned_ByteString (projT2 (fst (align_format_sumtype align_encoders st ce))),
-                      (snd (align_format_sumtype align_encoders st ce)))).
+                (ret (build_aligned_ByteString (projT2 (fst (align_format_sumtype align_encoders_n
+                                                                                  align_encoders_v
+                                                                                  align_encoders_ce st ce))),
+                      (snd (align_format_sumtype align_encoders_n
+                                                 align_encoders_v
+                                                 align_encoders_ce st ce)))).
   Proof.
     intros.
     etransitivity.
     eapply AlignedFormatDoneC.
-    rewrite (align_format_sumtype_OK A_OKs); try eassumption.
-    instantiate (2 := fun ce => fst (_ ce)).
-    instantiate (1 := fun ce => snd (_ ce)).
+    rewrite (align_format_sumtype_OK_inv A_OKs); try eassumption.
+    instantiate (2 := fun ce => fst (align_format_sumtype align_encoders_n align_encoders_v align_encoders_ce st ce)).
+    instantiate (1 := fun ce => snd (align_format_sumtype align_encoders_n align_encoders_v align_encoders_ce st ce)).
     simpl; reflexivity.
     simpl; reflexivity.
   Qed.
 
 End AlignedSumType.
+
+Arguments align_format_sumtype : simpl never.
+Arguments SumType_proj : simpl never.
+Arguments SumType_index : simpl never.
