src/Narcissus/Automation/Solver.v
@@ -43,6 +43,44 @@ Ltac apply_compose :=
 Ltac makeEvar T k :=
   let x := fresh in evar (x : T); let y := eval unfold x in x in clear x; k y.
 
+Ltac build_ilist_evar :=
+  match goal with
+  | |- appcontext[ith (m := ?n) (B := ?encT) (As := ?q ) ?z] =>
+    is_evar z;
+    match n with
+    | S ?n' => let T := eval simpl in (Vector.hd q) in
+                   makeEvar (encT T) ltac:(fun t' =>
+                                             let H' := match (type of (@icons _ encT T n' (Vector.tl q) t')) with
+                                                       | ?A -> _ => A
+                                                       end in
+                                             makeEvar H' ltac:(fun il' => unify z (@icons _ encT T n' (Vector.tl q) t' il')))
+    | _ => idtac
+    end
+  | |- context[icons (n := ?n) (B := ?encT) (l := ?q) ?a ?z] =>
+    is_evar z;
+    match n with
+    | S ?n' => let T := eval simpl in (Vector.hd q) in
+                   makeEvar (encT T) ltac:(fun t' =>
+                                             let H' := match (type of (@icons _ encT T n' (Vector.tl q) t')) with
+                                                       | ?A -> _ => A
+                                                       end in
+                                             makeEvar H' ltac:(fun il' => unify z (@icons _ encT T n' (Vector.tl q) t' il')))
+    | 0 => unify z (@inil _ encT)
+    end
+  end.
+
+Ltac build_prim_prod_evar :=
+  match goal with
+  | |- appcontext[ @ilist.prim_fst ?A unit ?z ?k] =>
+    is_evar z;
+    makeEvar A ltac:(fun a => unify z (Build_prim_prod a tt))
+  | |- appcontext[ @ilist.prim_fst ?A ?B ?z] =>
+    is_evar z;
+    makeEvar A ltac:(fun a =>
+                       makeEvar B ltac:(fun b =>
+                                          unify z (Build_prim_prod a b)))
+  end.
+
 Ltac shelve_inv :=
   let H' := fresh in
   let data := fresh in
